\documentclass[11pt]{article}
    \title{\textbf{Math 217 Homework I}}
    \author{Khac Nguyen Nguyen}
    \date{}
    
    \addtolength{\topmargin}{-3cm}
    \addtolength{\textheight}{3cm}
    
\usepackage{amsmath}
\usepackage{mathtools}
\usepackage{amsthm}
\usepackage{amssymb}
\usepackage{pgfplots}
\usepackage{xfrac}
\usepgfplotslibrary{polar}
\usepgflibrary{shapes.geometric}
\usetikzlibrary{calc}
\pgfplotsset{compat = newest}
\pgfplotsset{my style/.append style = {axis x line = middle, axis y line = middle, xlabel={$x$}, ylabel={$y$}, axis equal}}
\begin{document}
\section*{1.}
\begin{equation*}
    \begin{aligned}
        &P(T \in (-4,-2] \cup (-3,1) \cup [4,5) \cup [4.5,6)) \\
        =&\int_0^1  e^{-t} dt +\int_4^6 e^{-t} dt \\
        =& 0.647
    \end{aligned}
\end{equation*}
\pagebreak
\section*{2.}
\subsection*{a.}
Let $Y$ be the total time and $X$ be the amount of times we have to wait. Then we have that
\[
    E[Y] = E[E[Y|X]] = E\left[x \cdot \frac{1-0}{2}\right] = \frac{1}{2} E[X] 
    = \frac{1}{2} \cdot \frac{1}{\frac{1}{6}} = 3
\]
\subsection*{b.}
\[
    V[Y|X] = E[Y^2|X] - (E[Y|X])^2 = x \cdot E[Y_i^2] + x \cdot (x-1) E[Y_iY_j] = \frac{x}{12}
\]
since 
\[
    E[Y_i^2] = \int_0^1 y^2 dy = \frac{1}{3}    
\]
and 
\[
    E[Y_iY_j] = \left(\int_0^1 ydy\right)^2 = \frac{1}{4}    
\]
\[
    V[X] = \frac{1-\frac{1}{6}}{\frac{1}{6^2}} = 30 
\]
\[
    V[Y] = E[V[Y|X]] + V[E[Y|X]] = E[\frac{x}{12}] + V[0.5x] = \frac{1}{12} \cdot 6 + 0.25 \cdot 30 = 8    
\]
\pagebreak
\section*{3.}
\subsection*{a.}
As $\int 2z-2 dz = z^2 - 2z + C$, $C = 1$ so that $F_Z(1) = 0$ and $F_Z(2) = 1$. Hence,  we have
\[
    F_Z(z) = 
    \begin{cases}
        0 \indent & z<1 \\
        z^2-2z+1 \indent &1 \le z \le 2 \\
        1 \indent &z>2
    \end{cases}    
\]
\subsection*{b.}
Let $U(s)$ be the uniform random variable between 0 and 1, then 
\[
    V(s) = F^{-1}_X(U(s))    
\]
simulates the random variable.
\pagebreak
\section*{4.}
The inverse function that maps $\cfrac{e^{x^3}}{e^{x^3} + e^{-x^3}}$ to $x$. \\
We also have that 
\[
    \cfrac{e^{x^3}}{e^{x^3} + e^{x^{-3}}} = \cfrac{1}{1 + e^{-2x^3}}
\]
and hence 
\[
    \sqrt[3]{-\frac{1}{2}\ln\left(\cfrac{1}{\cfrac{e^{x^3}}{e^{x^3} + e^{-x^3}}}-1\right)} = x    
\]
which means that $F^{-1}_X$ is the function that maps $x$ to $\sqrt[3]{-\frac{1}{2}ln(\frac{1}{x}-1)}$ 
\subsection*{b.}
Let $U(s)$ be the uniform random variable between 0 and 1, then 
\[
    V(s) = F^{-1}_X(U(s))    
\]
simulates the random variable.
\end{document}