\documentclass[11pt]{article}
    \title{\textbf{Math 217 Homework I}}
    \author{Khac Nguyen Nguyen}
    \date{}
    
    \addtolength{\topmargin}{-3cm}
    \addtolength{\textheight}{3cm}
    
\usepackage{amsmath}
\usepackage{mathtools}
\usepackage{amsthm}
\usepackage{amssymb}
\usepackage{pgfplots}
\usepackage{xfrac}
\usepgfplotslibrary{polar}
\usepgflibrary{shapes.geometric}
\usetikzlibrary{calc}
\pgfplotsset{compat = newest}
\pgfplotsset{my style/.append style = {axis x line = middle, axis y line = middle, xlabel={$x$}, ylabel={$y$}, axis equal}}
\begin{document}
\section*{1.}
\[
    \int_0^b a(b-x) dx = \left.abx-\frac{ax^2}{2} \right|_0^b = \frac{ab^2}{2} = 1 \implies a = \frac{2}{b^2}
\]
\[
    E[X] = \int_0^b xa(b-x) dx = \left.\frac{abx^2}{2}- \frac{ax^3}{3} \right|_0^b = \frac{ab^3}{6} 
\]
\[
    E[X^2] = \int_0^b x^2a(b-x) dx = \left.\frac{abx^3}{3}- \frac{ax^4}{4} \right|_0^b = \frac{ab^4}{12}     
\]
Therefore, 
\[
    V[X] = E[X^2] - (E[X])^2 =  \frac{ab^4}{12} - \frac{a^2b^6}{36} = \frac{b^2}{6} - \frac{b^2}{9} = \frac{b^2}{18}  
\]
and hence 
\[
    \sigma_X = \frac{b\sqrt{2}}{6}    
\]
\[
    F(x) = \int ab-ax dx = abx - \frac{ax^2}{2} = \frac{2x}{b} - \frac{x^2}{b^2} + C      
\]
$C = 0$ so that $F(0) = 0$ and $F(b) = 1$. 
Therefore, 
\[
    P(X>E[X] + \sigma_X) = 1-F\left(\frac{2b + b\sqrt{2}}{6}\right) =     
\]
\pagebreak
\section*{2.}
\begin{equation*}
    \begin{aligned}
        M_X(t) 
        &= \frac{3}{2} \int_0^2 e^{tx} (x-1)^2 dx \\
        &= \frac{3}{2} \int_{-1}^1 e^{tx+t} x^2 dx \\
        &= \frac{3}{2} \left( \left. x^2 \cdot \frac{1}{t} e^{tx+t} \right|_{-1}^1 - \int_{-1}^1 \frac{2x}{t} e^{tx+t} dx \right)\\
        &= \frac{3}{2} \left( \frac{1}{t} e^{2t} - \frac{1}{t} - \left. \frac{2x}{t^2} e^{tx+t} \right|_{-1}^1 + \int_{-1}^1 \frac{2}{t^2} e^{tx+t} dx  \right)\\
        &= \frac{3}{2} \left( \frac{1}{t} e^{2t} - \frac{1}{t} - \frac{2}{t^2} e^{2t} - \frac{2}{t^2} + \left. \frac{2}{t^3} e^{tx+t} \right|_{-1}^1 \right) \\
        &= \frac{3}{2} \left( \frac{1}{t} e^{2t} - \frac{1}{t} - \frac{2}{t^2} e^{2t} - \frac{2}{t^2} + \frac{2e^{2t}}{t^3} - \frac{2}{t^3} \right) 
    \end{aligned}
\end{equation*}
\pagebreak
\section*{3.}
\begin{equation*}
    \begin{aligned}
        f(x) &= \frac{1}{3-x} \\
        &= \frac{1}{5} \cdot \frac{1}{1-\frac{1}{5}(2+x)} \\
        &= \frac{1}{5} \sum_{k=0}^\infty \left(\frac{1}{5}(2+x)\right)^k
    \end{aligned}
\end{equation*}
\pagebreak
\section*{4.}
\begin{equation*}
    \begin{aligned}
        E[N] &= \sum_{n=0}^\infty n \cdot 2 ^{-n-1} \\
        &= \sum_{n=0}^\infty (n-1) \cdot 2^{-n}  + 1  \\
        &= \sum_{n=0}^\infty n \cdot 2^{-n} + \sum_{n=0}^\infty 2^{-n} + 1 \\
        &= \frac{\frac{1}{2}}{\left(\frac{1}{2}-1\right)^2} - \frac{1}{1-\frac{1}{2}} + 1 \\
        &= 1
    \end{aligned}
\end{equation*}
\begin{equation*}
    \begin{aligned}
        E[N^2] &= \sum_{n=0}^\infty n^2 \cdot 2 ^{-n-1} \\
        &= \sum_{n=0}^\infty (n-1)^2 \cdot 2^{-n}  - 1  \\
        &= \sum_{n=0}^\infty n^2 \cdot 2^{-n} - 2 \sum_{n=0}^\infty n \cdot 2^{-n} + \sum_{n=0}^\infty 2^{-n} - 1 \\
        &= \frac{\frac{1}{2^2} + \frac{1}{2}}{\left(1-\frac{1}{2}\right)^3} - 2\cdot \frac{\frac{1}{2}}{\left(\frac{1}{2}-1\right)^2} + \frac{1}{1-\frac{1}{2}} - 1 \\
        &= 6 - 2\cdot 2 + 2 - 1 \\
        &= 3
    \end{aligned}
\end{equation*}
Hence, we have that 
\[
    V[N] = E[N^2] - (E[N])^2 = 2     
\]
We also have that 
\begin{equation*}
    \begin{aligned}
        V[Y] &= E[V[X|N]] + V[E[X|N]] \\
        &= E\left[\frac{1}{3} \cdot \frac{2}{3}\cdot n \right] + V\left[\frac{1}{3}n\right] \\
        &= \frac{2}{9} E[N] + \frac{1}{9} V[N] \\
        &= \frac{4}{9}
    \end{aligned}
\end{equation*}
\end{document}